@prefix :            <http://ns.nature.com/terms/> .
@prefix bibo:        <http://purl.org/ontology/bibo/> .
@prefix dc:          <http://purl.org/dc/elements/1.1/> .
@prefix dcterms:     <http://purl.org/dc/terms/> .
@prefix foaf:        <http://xmlns.com/foaf/0.1/> .
@prefix npg:         <http://ns.nature.com/terms/> .
@prefix npgd:        <http://ns.nature.com/datasets/> .
@prefix npgg:        <http://ns.nature.com/graphs/> .
@prefix owl:         <http://www.w3.org/2002/07/owl#> .
@prefix prism:       <http://prismstandard.org/namespaces/basic/2.1/> .
@prefix rdf:         <http://www.w3.org/1999/02/22-rdf-syntax-ns#> .
@prefix rdfs:        <http://www.w3.org/2000/01/rdf-schema#> .
@prefix skos:        <http://www.w3.org/2004/02/skos/core#> .
@prefix vann:        <http://purl.org/vocab/vann/> .
@prefix xsd:         <http://www.w3.org/2001/XMLSchema#> .

@prefix review-states: <http://ns.nature.com/review-states/> .

review-states:
    npg:webpage <http://www.nature.com/ontologies/models/review-states/> ;
    dc:date "2015-08-17T06:12:06.022-04:00" ;
    dc:publisher "Macmillan Publishers Limited" ;
    dc:rights "This work is distributed under a Creative Commons Zero 1.0 (CC0 1.0) Public Domain Dedication <http://creativecommons.org/publicdomain/zero/1.0/>."@en ;
    dcterms:license <http://creativecommons.org/publicdomain/zero/1.0/> ;
    vann:preferredNamespacePrefix "review-states" ;
    vann:preferredNamespaceUri "http://ns.nature.com/review-states/" ;
    a owl:Ontology, skos:ConceptScheme ;
    owl:imports <http://ns.nature.com/terms/> ;
    owl:versionInfo "1.9.45" ;
    skos:definition "The ReviewStates Ontology is a categorization of the various states that mark the review status of a publication."@en ;
    skos:prefLabel "ReviewStates Ontology"@en .

review-states:accepted
    npg:id "accepted" ;
    a npg:ReviewState , skos:Concept ;
    rdfs:isDefinedBy <http://ns.nature.com/review-states/> ;
    skos:definition "The :accepted review-state is used to characterize events in which an article is accepted for publication by a journal."@en ;
    skos:inScheme <http://ns.nature.com/review-states/> ;
    skos:prefLabel "Accepted"@en ;
    skos:topConceptOf <http://ns.nature.com/review-states/> .

review-states:created
    npg:id "created" ;
    a npg:ReviewState , skos:Concept ;
    rdfs:isDefinedBy <http://ns.nature.com/review-states/> ;
    skos:definition "The :created review-state is used to characterize events in which an article (typically a news item) is created on an internal system for a journal."@en ;
    skos:inScheme <http://ns.nature.com/review-states/> ;
    skos:prefLabel "Created"@en ;
    skos:topConceptOf <http://ns.nature.com/review-states/> .

review-states:first-decision
    npg:id "first-decision" ;
    a npg:ReviewState , skos:Concept ;
    rdfs:isDefinedBy <http://ns.nature.com/review-states/> ;
    skos:definition "The :first-decision review-state is used to characterize events in which a first decision on an article is made by a journal."@en ;
    skos:inScheme <http://ns.nature.com/review-states/> ;
    skos:prefLabel "First Decision"@en ;
    skos:topConceptOf <http://ns.nature.com/review-states/> .

review-states:received
    npg:id "received" ;
    a npg:ReviewState , skos:Concept ;
    rdfs:isDefinedBy <http://ns.nature.com/review-states/> ;
    skos:definition "The :received review-state is used to characterize events in which an article is received by a journal."@en ;
    skos:inScheme <http://ns.nature.com/review-states/> ;
    skos:prefLabel "Received"@en ;
    skos:topConceptOf <http://ns.nature.com/review-states/> .

review-states:revised
    npg:id "revised" ;
    a npg:ReviewState , skos:Concept ;
    rdfs:isDefinedBy <http://ns.nature.com/review-states/> ;
    skos:definition "The :revised review-state is used to characterize events in which a revision to an article is received by a journal."@en ;
    skos:inScheme <http://ns.nature.com/review-states/> ;
    skos:prefLabel "Revised"@en ;
    skos:topConceptOf <http://ns.nature.com/review-states/> .

